correctness/RegexCorrectness/Backtracker/Traversal/Lemmas.lean
@@ -3,7 +3,78 @@ import RegexCorrectness.Backtracker.Traversal.Invariants
 set_option autoImplicit false
 
 open Regex.Data (BitMatrix BoundedIterator)
+open String (Pos)
 
 namespace Regex.Backtracker
+
+namespace captureNextAux
+
+variable {nfa : NFA} {wf : nfa.WellFormed} {startIdx maxIdx : Nat} {bit₀ bit : BoundedIterator startIdx maxIdx}
+  {visited₀ visited : BitMatrix nfa.nodes.size (maxIdx + 1 - startIdx)} {stack : List (StackEntry HistoryStrategy nfa startIdx maxIdx)}
+
+theorem PathClosure.preserves {result} (hres : captureNextAux HistoryStrategy nfa wf startIdx maxIdx visited [⟨HistoryStrategy.empty, ⟨nfa.start, wf.start_lt⟩, bit⟩] = result)
+  (isNone : result.1 = .none) (v : bit.Valid) (isNextN : bit.IsNextNOf bit₀) (cls : PathClosure bit₀ visited) :
+  PathClosure bit₀ result.2 := by
+  have cinv : ClosureInv bit₀ visited [⟨HistoryStrategy.empty, ⟨nfa.start, wf.start_lt⟩, bit⟩] := by
+    intro state bit state' bit' update isNextN hmem step
+    exact .inl (cls state bit state' bit' (List.ofOption update) isNextN hmem (.last step))
+  exact path_closure hres isNone isNextN cinv (StackInv.intro v)
+
+theorem mem_or_path_of_mem_of_none {result} (hres : captureNextAux HistoryStrategy nfa wf startIdx maxIdx visited [⟨HistoryStrategy.empty, ⟨nfa.start, wf.start_lt⟩, bit⟩] = result)
+  (isNone : result.1 = .none) (v : bit.Valid) :
+  VisitedInv wf bit visited result.2 :=
+  visited_inv_of_none hres isNone VisitedInv.rfl (StackInv.intro v)
+
+theorem mem_of_path_of_none {result} (hres : captureNextAux HistoryStrategy nfa wf startIdx maxIdx visited [⟨HistoryStrategy.empty, ⟨nfa.start, wf.start_lt⟩, bit⟩] = result)
+  (isNone : result.1 = .none) (v : bit.Valid) (isNextN : bit.IsNextNOf bit₀) (cls : PathClosure bit₀ visited)
+  (bit' : BoundedIterator startIdx maxIdx) (state : Fin nfa.nodes.size) (update : List (Nat × Pos)) (path : Path nfa wf bit.it bit'.it state update) :
+  result.2.get state bit'.index := by
+  have mem_start : result.2.get ⟨nfa.start, wf.start_lt⟩ bit.index := hres ▸ mem_stack_top ⟨HistoryStrategy.empty, ⟨nfa.start, wf.start_lt⟩, bit⟩ [] rfl
+  match path.eq_or_nfaPath with
+  | .inl ⟨eqit, eqstate, _⟩ =>
+    have eq : bit' = bit := BoundedIterator.ext eqit
+    simpa [eq, ←eqstate] using mem_start
+  | .inr path =>
+    have cls' : PathClosure bit₀ result.2 := cls.preserves hres isNone v isNextN
+    exact cls' ⟨nfa.start, wf.start_lt⟩ bit state bit' update isNextN mem_start path
+
+theorem mem_iff_mem_or_path_of_none {result} (hres : captureNextAux HistoryStrategy nfa wf startIdx maxIdx visited [⟨HistoryStrategy.empty, ⟨nfa.start, wf.start_lt⟩, bit⟩] = result)
+  (isNone : result.1 = .none) (v : bit.Valid) (isNextN : bit.IsNextNOf bit₀) (cls : PathClosure bit₀ visited)
+  (bit' : BoundedIterator startIdx maxIdx) (state : Fin nfa.nodes.size) (isNextN' : bit'.IsNextNOf bit) :
+  result.2.get state bit'.index ↔ visited.get state bit'.index ∨ ∃ update, Path nfa wf bit.it bit'.it state update := by
+  apply Iff.intro
+  . intro mem
+    exact mem_or_path_of_mem_of_none hres isNone v state bit' isNextN' mem
+  . intro h
+    match h with
+    | .inl mem => exact hres ▸ mem_of_mem_visited mem
+    | .inr ⟨update, path⟩ => exact mem_of_path_of_none hres isNone v isNextN cls bit' state update path
+
+end captureNextAux
+
+namespace captureNext.go
+
+open captureNextAux (StackInv VisitedInv NotDoneInv)
+
+variable {nfa : NFA} {wf : nfa.WellFormed} {startIdx maxIdx : Nat} {bit₀ bit : BoundedIterator startIdx maxIdx} {visited₀ visited : BitMatrix nfa.nodes.size (maxIdx + 1 - startIdx)}
+
+theorem not_done_of_none {result} (hres : go HistoryStrategy nfa wf startIdx maxIdx bit visited = result)
+  (isNone : result.1 = .none)
+  (ndinv : NotDoneInv visited) :
+  NotDoneInv result.2 := by
+  induction bit, visited using captureNext.go.induct' HistoryStrategy nfa wf startIdx maxIdx with
+  | found bit visited update visited' haux =>
+    rw [captureNext.go_found haux] at hres
+    simp [←hres] at isNone
+  | not_found_next bit visited visited' haux hnext ih =>
+    rw [captureNext.go_not_found_next haux hnext] at hres
+    have ndinv' : NotDoneInv visited' := captureNextAux.not_done_of_none haux rfl ndinv
+    exact ih hres ndinv'
+  | not_found_end bit visited visited' haux hnext =>
+    rw [captureNext.go_not_found_end haux hnext] at hres
+    have ndinv' : NotDoneInv visited' := captureNextAux.not_done_of_none haux rfl ndinv
+    simpa [←hres] using ndinv'
+
+end captureNext.go
 
 end Regex.Backtracker
